src/goose_lang/notation.v
@@ -38,7 +38,7 @@ Notation LamV x e := (RecV BAnon x e) (only parsing).
 Notation LetCtx x e2 := (AppRCtx (LamV x e2)) (only parsing).
 Notation SeqCtx e2 := (LetCtx BAnon e2) (only parsing).
 Notation Match e0 x1 e1 x2 e2 := (Case e0 (Lam x1 e1) (Lam x2 e2)) (only parsing).
-Notation Alloc e := (AllocN (Val $ LitV $ LitInt (word.of_Z 1)) e) (only parsing).
+Notation Alloc e := (AllocN (Pair (Val $ LitV $ LitInt (U64 1)) e)) (only parsing).
 (** Compare-and-set (CAS) returns just a boolean indicating success or failure. *)
 Notation CAS l e1 e2 := (Snd (CmpXchg l e1 e2)) (only parsing).
 
@@ -117,7 +117,7 @@ Notation "~ e" := (UnOp NegOp e%E) (at level 75, right associativity) : expr_sco
 Definition Store {ext:ext_op} : val :=
   LamV "l" (Lam "v" (Seq
                      (PrepareWrite (Var "l"))
-                     (FinishStore (Var "l") (Var "v")))).
+                     (FinishStore (Pair (Var "l") (Var "v"))))).
 (* The unicode ← is already part of the notation "_ ← _; _" for bind. *)
 Notation "e1 <- e2" := (Store e1%E e2%E) (at level 80) : expr_scope.
 
